Codegen main

SimPro.sml
@@ -1,11 +1,11 @@
 structure SimPro : sig
   type nat
-  type nibble
-  type char
   type nnf
+  val main :
+    ((((nat * nnf) list) list -> ((nat * nnf) list) list) ->
+      ((nat * nnf) list) list -> bool) ->
+      nnf -> bool
   val test : nnf
-  val make_sequents : nnf -> ((nat * nnf) list) list
-  val next_sequents : ((nat * nnf) list) list -> ((nat * nnf) list) list
 end = struct
 
 datatype nat = Zero_nat | Suc of nat;
@@ -33,276 +33,8 @@ fun equal_list A_ [] (x21 :: x22) = false
     eq A_ x21 y21 andalso equal_list A_ x22 y22
   | equal_list A_ [] [] = true;
 
-datatype nibble = Nibble0 | Nibble1 | Nibble2 | Nibble3 | Nibble4 | Nibble5 |
-  Nibble6 | Nibble7 | Nibble8 | Nibble9 | NibbleA | NibbleB | NibbleC | NibbleD
-  | NibbleE | NibbleF;
-
-datatype char = Char of nibble * nibble;
-
-datatype nnf = Pre of bool * char list * nat list | Con of nnf * nnf |
+datatype nnf = Pre of bool * nat * nat list | Con of nnf * nnf |
   Dis of nnf * nnf | Uni of nnf | Exi of nnf;
-
-fun equal_nibble NibbleE NibbleF = false
-  | equal_nibble NibbleF NibbleE = false
-  | equal_nibble NibbleD NibbleF = false
-  | equal_nibble NibbleF NibbleD = false
-  | equal_nibble NibbleD NibbleE = false
-  | equal_nibble NibbleE NibbleD = false
-  | equal_nibble NibbleC NibbleF = false
-  | equal_nibble NibbleF NibbleC = false
-  | equal_nibble NibbleC NibbleE = false
-  | equal_nibble NibbleE NibbleC = false
-  | equal_nibble NibbleC NibbleD = false
-  | equal_nibble NibbleD NibbleC = false
-  | equal_nibble NibbleB NibbleF = false
-  | equal_nibble NibbleF NibbleB = false
-  | equal_nibble NibbleB NibbleE = false
-  | equal_nibble NibbleE NibbleB = false
-  | equal_nibble NibbleB NibbleD = false
-  | equal_nibble NibbleD NibbleB = false
-  | equal_nibble NibbleB NibbleC = false
-  | equal_nibble NibbleC NibbleB = false
-  | equal_nibble NibbleA NibbleF = false
-  | equal_nibble NibbleF NibbleA = false
-  | equal_nibble NibbleA NibbleE = false
-  | equal_nibble NibbleE NibbleA = false
-  | equal_nibble NibbleA NibbleD = false
-  | equal_nibble NibbleD NibbleA = false
-  | equal_nibble NibbleA NibbleC = false
-  | equal_nibble NibbleC NibbleA = false
-  | equal_nibble NibbleA NibbleB = false
-  | equal_nibble NibbleB NibbleA = false
-  | equal_nibble Nibble9 NibbleF = false
-  | equal_nibble NibbleF Nibble9 = false
-  | equal_nibble Nibble9 NibbleE = false
-  | equal_nibble NibbleE Nibble9 = false
-  | equal_nibble Nibble9 NibbleD = false
-  | equal_nibble NibbleD Nibble9 = false
-  | equal_nibble Nibble9 NibbleC = false
-  | equal_nibble NibbleC Nibble9 = false
-  | equal_nibble Nibble9 NibbleB = false
-  | equal_nibble NibbleB Nibble9 = false
-  | equal_nibble Nibble9 NibbleA = false
-  | equal_nibble NibbleA Nibble9 = false
-  | equal_nibble Nibble8 NibbleF = false
-  | equal_nibble NibbleF Nibble8 = false
-  | equal_nibble Nibble8 NibbleE = false
-  | equal_nibble NibbleE Nibble8 = false
-  | equal_nibble Nibble8 NibbleD = false
-  | equal_nibble NibbleD Nibble8 = false
-  | equal_nibble Nibble8 NibbleC = false
-  | equal_nibble NibbleC Nibble8 = false
-  | equal_nibble Nibble8 NibbleB = false
-  | equal_nibble NibbleB Nibble8 = false
-  | equal_nibble Nibble8 NibbleA = false
-  | equal_nibble NibbleA Nibble8 = false
-  | equal_nibble Nibble8 Nibble9 = false
-  | equal_nibble Nibble9 Nibble8 = false
-  | equal_nibble Nibble7 NibbleF = false
-  | equal_nibble NibbleF Nibble7 = false
-  | equal_nibble Nibble7 NibbleE = false
-  | equal_nibble NibbleE Nibble7 = false
-  | equal_nibble Nibble7 NibbleD = false
-  | equal_nibble NibbleD Nibble7 = false
-  | equal_nibble Nibble7 NibbleC = false
-  | equal_nibble NibbleC Nibble7 = false
-  | equal_nibble Nibble7 NibbleB = false
-  | equal_nibble NibbleB Nibble7 = false
-  | equal_nibble Nibble7 NibbleA = false
-  | equal_nibble NibbleA Nibble7 = false
-  | equal_nibble Nibble7 Nibble9 = false
-  | equal_nibble Nibble9 Nibble7 = false
-  | equal_nibble Nibble7 Nibble8 = false
-  | equal_nibble Nibble8 Nibble7 = false
-  | equal_nibble Nibble6 NibbleF = false
-  | equal_nibble NibbleF Nibble6 = false
-  | equal_nibble Nibble6 NibbleE = false
-  | equal_nibble NibbleE Nibble6 = false
-  | equal_nibble Nibble6 NibbleD = false
-  | equal_nibble NibbleD Nibble6 = false
-  | equal_nibble Nibble6 NibbleC = false
-  | equal_nibble NibbleC Nibble6 = false
-  | equal_nibble Nibble6 NibbleB = false
-  | equal_nibble NibbleB Nibble6 = false
-  | equal_nibble Nibble6 NibbleA = false
-  | equal_nibble NibbleA Nibble6 = false
-  | equal_nibble Nibble6 Nibble9 = false
-  | equal_nibble Nibble9 Nibble6 = false
-  | equal_nibble Nibble6 Nibble8 = false
-  | equal_nibble Nibble8 Nibble6 = false
-  | equal_nibble Nibble6 Nibble7 = false
-  | equal_nibble Nibble7 Nibble6 = false
-  | equal_nibble Nibble5 NibbleF = false
-  | equal_nibble NibbleF Nibble5 = false
-  | equal_nibble Nibble5 NibbleE = false
-  | equal_nibble NibbleE Nibble5 = false
-  | equal_nibble Nibble5 NibbleD = false
-  | equal_nibble NibbleD Nibble5 = false
-  | equal_nibble Nibble5 NibbleC = false
-  | equal_nibble NibbleC Nibble5 = false
-  | equal_nibble Nibble5 NibbleB = false
-  | equal_nibble NibbleB Nibble5 = false
-  | equal_nibble Nibble5 NibbleA = false
-  | equal_nibble NibbleA Nibble5 = false
-  | equal_nibble Nibble5 Nibble9 = false
-  | equal_nibble Nibble9 Nibble5 = false
-  | equal_nibble Nibble5 Nibble8 = false
-  | equal_nibble Nibble8 Nibble5 = false
-  | equal_nibble Nibble5 Nibble7 = false
-  | equal_nibble Nibble7 Nibble5 = false
-  | equal_nibble Nibble5 Nibble6 = false
-  | equal_nibble Nibble6 Nibble5 = false
-  | equal_nibble Nibble4 NibbleF = false
-  | equal_nibble NibbleF Nibble4 = false
-  | equal_nibble Nibble4 NibbleE = false
-  | equal_nibble NibbleE Nibble4 = false
-  | equal_nibble Nibble4 NibbleD = false
-  | equal_nibble NibbleD Nibble4 = false
-  | equal_nibble Nibble4 NibbleC = false
-  | equal_nibble NibbleC Nibble4 = false
-  | equal_nibble Nibble4 NibbleB = false
-  | equal_nibble NibbleB Nibble4 = false
-  | equal_nibble Nibble4 NibbleA = false
-  | equal_nibble NibbleA Nibble4 = false
-  | equal_nibble Nibble4 Nibble9 = false
-  | equal_nibble Nibble9 Nibble4 = false
-  | equal_nibble Nibble4 Nibble8 = false
-  | equal_nibble Nibble8 Nibble4 = false
-  | equal_nibble Nibble4 Nibble7 = false
-  | equal_nibble Nibble7 Nibble4 = false
-  | equal_nibble Nibble4 Nibble6 = false
-  | equal_nibble Nibble6 Nibble4 = false
-  | equal_nibble Nibble4 Nibble5 = false
-  | equal_nibble Nibble5 Nibble4 = false
-  | equal_nibble Nibble3 NibbleF = false
-  | equal_nibble NibbleF Nibble3 = false
-  | equal_nibble Nibble3 NibbleE = false
-  | equal_nibble NibbleE Nibble3 = false
-  | equal_nibble Nibble3 NibbleD = false
-  | equal_nibble NibbleD Nibble3 = false
-  | equal_nibble Nibble3 NibbleC = false
-  | equal_nibble NibbleC Nibble3 = false
-  | equal_nibble Nibble3 NibbleB = false
-  | equal_nibble NibbleB Nibble3 = false
-  | equal_nibble Nibble3 NibbleA = false
-  | equal_nibble NibbleA Nibble3 = false
-  | equal_nibble Nibble3 Nibble9 = false
-  | equal_nibble Nibble9 Nibble3 = false
-  | equal_nibble Nibble3 Nibble8 = false
-  | equal_nibble Nibble8 Nibble3 = false
-  | equal_nibble Nibble3 Nibble7 = false
-  | equal_nibble Nibble7 Nibble3 = false
-  | equal_nibble Nibble3 Nibble6 = false
-  | equal_nibble Nibble6 Nibble3 = false
-  | equal_nibble Nibble3 Nibble5 = false
-  | equal_nibble Nibble5 Nibble3 = false
-  | equal_nibble Nibble3 Nibble4 = false
-  | equal_nibble Nibble4 Nibble3 = false
-  | equal_nibble Nibble2 NibbleF = false
-  | equal_nibble NibbleF Nibble2 = false
-  | equal_nibble Nibble2 NibbleE = false
-  | equal_nibble NibbleE Nibble2 = false
-  | equal_nibble Nibble2 NibbleD = false
-  | equal_nibble NibbleD Nibble2 = false
-  | equal_nibble Nibble2 NibbleC = false
-  | equal_nibble NibbleC Nibble2 = false
-  | equal_nibble Nibble2 NibbleB = false
-  | equal_nibble NibbleB Nibble2 = false
-  | equal_nibble Nibble2 NibbleA = false
-  | equal_nibble NibbleA Nibble2 = false
-  | equal_nibble Nibble2 Nibble9 = false
-  | equal_nibble Nibble9 Nibble2 = false
-  | equal_nibble Nibble2 Nibble8 = false
-  | equal_nibble Nibble8 Nibble2 = false
-  | equal_nibble Nibble2 Nibble7 = false
-  | equal_nibble Nibble7 Nibble2 = false
-  | equal_nibble Nibble2 Nibble6 = false
-  | equal_nibble Nibble6 Nibble2 = false
-  | equal_nibble Nibble2 Nibble5 = false
-  | equal_nibble Nibble5 Nibble2 = false
-  | equal_nibble Nibble2 Nibble4 = false
-  | equal_nibble Nibble4 Nibble2 = false
-  | equal_nibble Nibble2 Nibble3 = false
-  | equal_nibble Nibble3 Nibble2 = false
-  | equal_nibble Nibble1 NibbleF = false
-  | equal_nibble NibbleF Nibble1 = false
-  | equal_nibble Nibble1 NibbleE = false
-  | equal_nibble NibbleE Nibble1 = false
-  | equal_nibble Nibble1 NibbleD = false
-  | equal_nibble NibbleD Nibble1 = false
-  | equal_nibble Nibble1 NibbleC = false
-  | equal_nibble NibbleC Nibble1 = false
-  | equal_nibble Nibble1 NibbleB = false
-  | equal_nibble NibbleB Nibble1 = false
-  | equal_nibble Nibble1 NibbleA = false
-  | equal_nibble NibbleA Nibble1 = false
-  | equal_nibble Nibble1 Nibble9 = false
-  | equal_nibble Nibble9 Nibble1 = false
-  | equal_nibble Nibble1 Nibble8 = false
-  | equal_nibble Nibble8 Nibble1 = false
-  | equal_nibble Nibble1 Nibble7 = false
-  | equal_nibble Nibble7 Nibble1 = false
-  | equal_nibble Nibble1 Nibble6 = false
-  | equal_nibble Nibble6 Nibble1 = false
-  | equal_nibble Nibble1 Nibble5 = false
-  | equal_nibble Nibble5 Nibble1 = false
-  | equal_nibble Nibble1 Nibble4 = false
-  | equal_nibble Nibble4 Nibble1 = false
-  | equal_nibble Nibble1 Nibble3 = false
-  | equal_nibble Nibble3 Nibble1 = false
-  | equal_nibble Nibble1 Nibble2 = false
-  | equal_nibble Nibble2 Nibble1 = false
-  | equal_nibble Nibble0 NibbleF = false
-  | equal_nibble NibbleF Nibble0 = false
-  | equal_nibble Nibble0 NibbleE = false
-  | equal_nibble NibbleE Nibble0 = false
-  | equal_nibble Nibble0 NibbleD = false
-  | equal_nibble NibbleD Nibble0 = false
-  | equal_nibble Nibble0 NibbleC = false
-  | equal_nibble NibbleC Nibble0 = false
-  | equal_nibble Nibble0 NibbleB = false
-  | equal_nibble NibbleB Nibble0 = false
-  | equal_nibble Nibble0 NibbleA = false
-  | equal_nibble NibbleA Nibble0 = false
-  | equal_nibble Nibble0 Nibble9 = false
-  | equal_nibble Nibble9 Nibble0 = false
-  | equal_nibble Nibble0 Nibble8 = false
-  | equal_nibble Nibble8 Nibble0 = false
-  | equal_nibble Nibble0 Nibble7 = false
-  | equal_nibble Nibble7 Nibble0 = false
-  | equal_nibble Nibble0 Nibble6 = false
-  | equal_nibble Nibble6 Nibble0 = false
-  | equal_nibble Nibble0 Nibble5 = false
-  | equal_nibble Nibble5 Nibble0 = false
-  | equal_nibble Nibble0 Nibble4 = false
-  | equal_nibble Nibble4 Nibble0 = false
-  | equal_nibble Nibble0 Nibble3 = false
-  | equal_nibble Nibble3 Nibble0 = false
-  | equal_nibble Nibble0 Nibble2 = false
-  | equal_nibble Nibble2 Nibble0 = false
-  | equal_nibble Nibble0 Nibble1 = false
-  | equal_nibble Nibble1 Nibble0 = false
-  | equal_nibble NibbleF NibbleF = true
-  | equal_nibble NibbleE NibbleE = true
-  | equal_nibble NibbleD NibbleD = true
-  | equal_nibble NibbleC NibbleC = true
-  | equal_nibble NibbleB NibbleB = true
-  | equal_nibble NibbleA NibbleA = true
-  | equal_nibble Nibble9 Nibble9 = true
-  | equal_nibble Nibble8 Nibble8 = true
-  | equal_nibble Nibble7 Nibble7 = true
-  | equal_nibble Nibble6 Nibble6 = true
-  | equal_nibble Nibble5 Nibble5 = true
-  | equal_nibble Nibble4 Nibble4 = true
-  | equal_nibble Nibble3 Nibble3 = true
-  | equal_nibble Nibble2 Nibble2 = true
-  | equal_nibble Nibble1 Nibble1 = true
-  | equal_nibble Nibble0 Nibble0 = true;
-
-fun equal_chara (Char (x1, x2)) (Char (y1, y2)) =
-  equal_nibble x1 y1 andalso equal_nibble x2 y2;
-
-val equal_char = {equal = equal_chara} : char equal;
 
 fun equal_nnfa (Uni x4) (Exi x5) = false
   | equal_nnfa (Exi x5) (Uni x4) = false
@@ -332,7 +64,7 @@ fun equal_nnfa (Uni x4) (Exi x5) = false
     equal_nnfa x21 y21 andalso equal_nnfa x22 y22
   | equal_nnfa (Pre (x11, x12, x13)) (Pre (y11, y12, y13)) =
     equal_bool x11 y11 andalso
-      (equal_list equal_char x12 y12 andalso equal_list equal_nat x13 y13);
+      (equal_nata x12 y12 andalso equal_list equal_nat x13 y13);
 
 val equal_nnf = {equal = equal_nnfa} : nnf equal;
 
@@ -371,13 +103,15 @@ fun subst f (Pre (b, i, v)) = Pre (b, i, map f v)
 
 fun inst p n = subst (bind n) p;
 
-fun mapsa f l = maps f l;
+fun snd (x1, x2) = x2;
 
-fun maxd Zero_nat = Zero_nat
-  | maxd (Suc n) = n;
+fun fst (x1, x2) = x1;
 
 fun maxp x Zero_nat = x
   | maxp x (Suc n) = Suc (maxp x n);
+
+fun maxd Zero_nat = Zero_nat
+  | maxd (Suc n) = n;
 
 fun maxm x Zero_nat = x
   | maxm x (Suc n) = maxm (maxd x) n;
@@ -385,20 +119,12 @@ fun maxm x Zero_nat = x
 fun maxl [] = Zero_nat
   | maxl (h :: t) = maxp (maxm (maxl t) h) h;
 
+fun fresh l = (if null l then Zero_nat else Suc (maxl l));
+
 fun stop B_ a uu [] = a
   | stop B_ a p (h :: t) = (if eq B_ p h then [] else stop B_ a p t);
 
-val test : nnf =
-  Dis (Uni (Con (Pre (false, [Char (Nibble5, Nibble0)], [Zero_nat]),
-                  Pre (false, [Char (Nibble5, Nibble1)], [Zero_nat]))),
-        Dis (Exi (Pre (true, [Char (Nibble5, Nibble1)], [Zero_nat])),
-              Exi (Pre (true, [Char (Nibble5, Nibble0)], [Zero_nat]))));
-
-fun fresh l = (if null l then Zero_nat else Suc (maxl l));
-
-fun snd (x1, x2) = x2;
-
-fun fst (x1, x2) = x1;
+fun mapsa f l = maps f l;
 
 fun track s uu (Pre (b, i, v)) =
   stop equal_nnf [s @ [(Zero_nat, Pre (b, i, v))]] (Pre (not b, i, v))
@@ -412,8 +138,12 @@ fun track s uu (Pre (b, i, v)) =
 fun solve [] = [[]]
   | solve (h :: t) = track t (fst h) (snd h);
 
-fun make_sequents p = [[(Zero_nat, p)]];
+fun main prover p = prover (mapsa solve) [[(Zero_nat, p)]];
 
-fun next_sequents a = mapsa solve a;
+val test : nnf =
+  Dis (Uni (Con (Pre (false, Zero_nat, [Zero_nat]),
+                  Pre (false, Suc Zero_nat, [Zero_nat]))),
+        Dis (Exi (Pre (true, Suc Zero_nat, [Zero_nat])),
+              Exi (Pre (true, Zero_nat, [Zero_nat]))));
 
 end; (*struct SimPro*)
